src/program_proof/memkv/memkv_coord_ghost_init.v
@@ -10,9 +10,10 @@ Section memkv_coord_ghost_init_proof.
 (* These lemmas happen *before* we get node local names (e.g. the gname for memory, crashes etc. *)
 Context `{!gooseGlobalGS Σ, erpcG Σ, urpcregG Σ, kvMapG Σ}.
 
-Definition coord_SpecList γkv : plist (u64 * RpcSpec) :=
-  pcons (U64 uCOORD_ADD, is_coord_server_addSpec γkv)
-    (pcons (U64 uCOORD_GET, is_coord_server_getSpec γkv) pnil).
+Definition coord_SpecList γkv : plist (pprod u64 RpcSpec) :=
+  pcons (ppair (U64 uCOORD_ADD) (is_coord_server_addSpec γkv))
+  $ pcons (ppair (U64 uCOORD_GET) (is_coord_server_getSpec γkv))
+  $ pnil.
 
 Lemma coord_server_ghost_init host (γkv : gname) :
   host c↦ ∅ ={⊤}=∗
